internal/Notations.v
@@ -1,7 +1,18 @@
 Reserved Notation "x ‘‘→’’ y" (at level 99, right associativity, y at level 200).
 Reserved Notation "x ‘→’ y" (at level 99, right associativity, y at level 200).
 Reserved Notation "x ‘’ y" (at level 15, left associativity).
+Reserved Notation "x ‘’₀ y" (at level 15, left associativity).
+Reserved Notation "x ‘’₁ y" (at level 15, left associativity).
+Reserved Notation "x ‘’₂ y" (at level 15, left associativity).
+Reserved Notation "x ‘’₃ y" (at level 15, left associativity).
+Reserved Notation "x ‘’₄ y" (at level 15, left associativity).
+Reserved Notation "x ‘’₅ y" (at level 15, left associativity).
+Reserved Notation "x ‘’₆ y" (at level 15, left associativity).
+Reserved Notation "x ‘’₇ y" (at level 15, left associativity).
+Reserved Notation "x ‘’₈ y" (at level 15, left associativity).
+Reserved Notation "x ‘’₉ y" (at level 15, left associativity).
 Reserved Notation "x ‘‘’’ y" (at level 15, left associativity).
+Reserved Notation "x ‘‘’’₅ y" (at level 15, left associativity).
 Reserved Notation "Γ ▻ x" (at level 65, left associativity).
 Reserved Notation "Γ ▻▻ Γ'" (at level 65, left associativity).
 Reserved Notation "Γ ‘▻’ x" (at level 65, left associativity).
